casestudies/compcert/lib/Prelude.v
@@ -1,0 +1,21 @@
+Require Import Orders.
+Require Import Mergesort.
+Require Import Ordered.
+From NFPOP Require Import Coqlib.
+From NFPOP Require Import AST.
+Require Import Coq.ZArith.ZArith.
+
+Axiom cheat : forall {X}, X.
+
+Module VarOrder <: TotalLeBool.
+  Definition t := (ident * Z)%type.
+  Definition leb (v1 v2: t) : bool := zle (snd v1) (snd v2).
+  Theorem leb_total: forall v1 v2, leb v1 v2 = true \/ leb v2 v1 = true.
+  Proof.
+    unfold leb; intros.
+    assert (snd v1 <= snd v2 \/ snd v2 <= snd v1) by lia.
+    unfold proj_sumbool. destruct H; [left|right]; apply zle_true; auto.
+  Qed.
+End VarOrder.
+
+Module VarSort := Mergesort.Sort(VarOrder).
